Prove that retcall elim and seq assoc preserve evaluation

pancake/semantics/panSemScript.sml
@@ -310,13 +310,15 @@ Definition evaluate_def:
      | SOME (ValWord w) =>
        if (w <> 0w) then
         let (res,s1) = fix_clock s (evaluate (c,s)) in
+        case res of
+        | SOME Continue =>
+            if s1.clock = 0 then (SOME TimeOut,empty_locals s1)
+            else evaluate (While e c,dec_clock s1)
+        | NONE =>
           if s1.clock = 0 then (SOME TimeOut,empty_locals s1)
-          else
-           case res of
-            | SOME Continue => evaluate (While e c,dec_clock s1)
-            | NONE => evaluate (While e c,dec_clock s1)
-            | SOME Break => (NONE,s1)
-            | _ => (res,s1)
+          else evaluate (While e c,dec_clock s1)
+        | SOME Break => (NONE,s1)
+        | _ => (res,s1)
        else (NONE,s)
        | _ => (SOME Error,s)) /\
   (evaluate (Return e,s) =
@@ -414,16 +416,15 @@ Theorem evaluate_clock:
    !prog s r s'. (evaluate (prog,s) = (r,s')) ==>
                  s'.clock <= s.clock
 Proof
-  (*recInduct evaluate_ind \\ REPEAT STRIP_TAC
-  \\ POP_ASSUM MP_TAC \\ ONCE_REWRITE_TAC [evaluate_def]
-  \\ rw [] \\ every_case_tac
-  \\ fs [set_var_def, mem_store_def,call_env_def,dec_clock_def, LET_THM]
-  \\ rveq \\ fs []
-  \\ rpt (pairarg_tac \\ fs [])
-  \\ every_case_tac \\ fs [] \\ rveq
-  \\ imp_res_tac fix_clock_IMP_LESS_EQ
-  \\ imp_res_tac LESS_EQ_TRANS \\ fs []*)
- cheat
+  recInduct evaluate_ind >> REPEAT STRIP_TAC >>
+  POP_ASSUM MP_TAC >> ONCE_REWRITE_TAC [evaluate_def] >>
+  rw [] >> every_case_tac >>
+  fs [set_var_def, upd_locals_def, empty_locals_def, dec_clock_def, LET_THM] >>
+  rveq >> fs [] >>
+  rpt (pairarg_tac >> fs []) >>
+  every_case_tac >> fs [] >> rveq >>
+  imp_res_tac fix_clock_IMP_LESS_EQ >>
+  imp_res_tac LESS_EQ_TRANS >> fs [] >> rfs []
 QED
 
 Theorem fix_clock_evaluate:
